examples/Imp2Vir/CvirCombinatorsWF.v
@@ -27,7 +27,7 @@ Definition unique_bid {ni no} ir : Prop :=
   b1 = b2.
 
 Theorem nth_firstn : forall A (l : list A) i n a,
-  i < n -> List.nth i (firstn n l) a = List.nth i l a.
+  i < n -> List.nth i (List.firstn n l) a = List.nth i l a.
 Proof.
   induction l ; intros.
   - rewrite firstn_nil. reflexivity.
@@ -47,11 +47,10 @@ Definition out_blk_id id (b : block typ) : Prop :=
 
 Definition cvir_ids_WF {ni no} ir : Prop :=
   forall (vi : Vec.t raw_id ni) (vo : Vec.t raw_id no) vt b,
+  List.In b (blocks ir vi vo vt) ->
   (
-    List.In b (blocks ir vi vo vt) ->
     In (blk_id b) (vi ++ vt)%vec
   ) /\ (
-    List.In b (blocks ir vi vo vt) ->
     forall bid,
     out_blk_id bid b ->
     In bid (vo ++ vt)%vec
@@ -84,6 +83,54 @@ Proof.
     unfold Vec.hd. simpl. intuition.
 Qed.
 
+Theorem block_cvir_unique : forall c, unique_bid (block_cvir c).
+Proof.
+  unfold unique_bid, block_cvir.
+  simpl.
+  intros.
+  intuition.
+  subst.
+  reflexivity.
+Qed.
+
+Theorem branch_cvir_id_WF : forall c e, cvir_ids_WF (branch_cvir c e).
+Proof.
+  unfold cvir_ids_WF.
+  intros ? ? [] [] [].
+  split ; intros.
+  - simpl in H.
+    destruct H ; [| contradiction ].
+    apply vector_in_app_iff.
+    left.
+    unfold In.
+    subst.
+    simpl.
+    destruct x ; simpl in * ; [lia |].
+    unfold Vec.hd. simpl. intuition.
+  - unfold out_blk_id in H0.
+    simpl in *.
+    destruct H ; [| contradiction ].
+    apply vector_in_app_iff.
+    left.
+    unfold In.
+    subst.
+    simpl in *.
+    subst.
+    destruct x0 ; simpl in * ; [lia |].
+    destruct x0 ; simpl in * ; [lia |].
+    unfold Vec.hd in *. simpl in *. intuition.
+Qed.
+
+Theorem branch_cvir_unique : forall c e, unique_bid (branch_cvir c e).
+Proof.
+  unfold unique_bid, block_cvir.
+  simpl.
+  intros.
+  intuition.
+  subst.
+  reflexivity.
+Qed.
+
 Theorem unique_vector_reorder :
   forall A n1 n2 n3 n4 (v1 : Vec.t A n1) (v2 : Vec.t A n2) (v3 : Vec.t A n3) (v4 : Vec.t A n4),
   unique_vector ((v1 ++ v2) ++ v3 ++ v4) -> unique_vector ((v1 ++ v3) ++ v2 ++ v4).
@@ -105,21 +152,19 @@ Theorem merge_cvir_id_WF :
   cvir_ids_WF (merge_cvir ir1 ir2).
 Proof.
   unfold cvir_ids_WF.
-  intros ? ? ? ? ? ? ? ? ? ? ? ?.
+  intros ? ? ? ? ? ? ? ? ? ? ? ? ?.
   split_vec vi ni1.
   split_vec vo no1.
   split_vec vt (n_int ir1).
   Opaque Vec.splitat.
   simpl in *.
-  rewrite 3 splitat_append.
-  edestruct H, H0.
-  rewrite vector_in_app_iff in H1, H3.
-  split ; intros ; rewrite 3 vector_in_app_iff ; apply in_app_iff in H5.
-  - destruct H5 ; apply H1 in H5 + apply H3 in H5 ; destruct H5 ; intuition.
-  - destruct H5 ; eapply H2 in H5 + eapply H4 in H5.
-    2, 4: eassumption.
-    all: rewrite vector_in_app_iff in H5.
-    all: intuition.
+  rewrite 3 splitat_append in H1.
+  apply in_app_iff in H1.
+  split ; intros ; rewrite 3 vector_in_app_iff.
+  - destruct H1 ; apply H in H1 + apply H0 in H1 ;
+    rewrite vector_in_app_iff in H1 ; intuition.
+  - destruct H1 ; apply H in H1 + apply H0 in H1 ; apply H1 in H2 ;
+    rewrite vector_in_app_iff in H2 ; intuition.
 Qed.
 
 Theorem merge_cvir_blocks :
@@ -156,6 +201,7 @@ Proof.
     all: assumption.
   - apply H in H4.
     apply H0 in H5.
+    destruct H4 as [? _], H5 as [? _].
     eapply In_nth in H4, H5.
     destruct H4 as [? ?], H5 as [? ?].
     erewrite <- vector_app_nth1 in H4.
@@ -169,6 +215,7 @@ Proof.
     lia.
   - apply H0 in H4.
     apply H in H5.
+    destruct H4 as [? _], H5 as [? _].
     eapply In_nth in H4, H5.
     destruct H4 as [? ?], H5 as [? ?].
     erewrite <- vector_app_nth2 in H4.
@@ -185,80 +232,203 @@ Proof.
     all: assumption.
 Qed.
 
+Theorem sym_i_cvir_id_WF :
+  forall ni1 ni2 ni3 no (ir : cvir (ni1+(ni2+ni3)) no),
+  cvir_ids_WF ir -> cvir_ids_WF (sym_i_cvir ir).
+Proof.
+  unfold cvir_ids_WF. intros.
+  unfold sym_i_cvir in H0.
+  split_vec vi ni1.
+  split_vec vi2 ni3.
+  rename vi21 into vi2, vi22 into vi3.
+  simpl in H0.
+  rewrite sym_vec_app in H0.
+  apply H in H0.
+  unfold In in H0.
+  simpl in H0.
+  rewrite 3 in_app_iff in H0.
+  rewrite 3 vector_in_app_iff.
+  intuition.
+Qed.
+
+Theorem sym_i_cvir_unique :
+  forall ni1 ni2 ni3 no (ir : cvir (ni1+(ni2+ni3)) no),
+  unique_bid ir ->
+  unique_bid (sym_i_cvir ir).
+Proof.
+  unfold unique_bid.
+  intros.
+  split_vec vi ni1.
+  split_vec vi2 ni3.
+  rename vi21 into vi2, vi22 into vi3.
+  eapply H. 4: apply H3. 3: apply H2. 2: apply H1.
+  rewrite sym_vec_app.
+  apply unique_list_vector. apply unique_list_vector in H0. simpl in *.
+  rewrite <- app_assoc. rewrite <- app_assoc. apply unique_list_sym2.
+  rewrite <- app_assoc. rewrite app_assoc. apply unique_list_sym2.
+  rewrite <- app_assoc. rewrite <- 2 app_assoc in H0. exact H0.
+Qed.
+
+Theorem cast_i_cvir_id_WF :
+  forall ni ni' no (ir : cvir ni no) (H : ni = ni'),
+  cvir_ids_WF ir -> cvir_ids_WF (cast_i_cvir ir H).
+Proof.
+  unfold cvir_ids_WF. intros.
+  simpl in H1.
+  destruct vi.
+  simpl in H1.
+  apply H0 in H1.
+  apply H1.
+Qed.
+
+Theorem cast_o_cvir_id_WF :
+  forall ni no no' (ir : cvir ni no) (H : no = no'),
+  cvir_ids_WF ir -> cvir_ids_WF (cast_o_cvir ir H).
+Proof.
+  unfold cvir_ids_WF. intros.
+  simpl in H1.
+  destruct vi.
+  simpl in H1.
+  apply H0 in H1.
+  apply H1.
+Qed.
+
+Theorem cast_i_cvir_unique :
+  forall ni ni' no (ir : cvir ni no) (H : ni = ni'),
+  unique_bid ir -> unique_bid (cast_i_cvir ir H).
+Proof.
+  unfold unique_bid. intros.
+  destruct vi.
+  simpl in *.
+  eapply H0 ; try eassumption.
+  apply unique_list_vector.
+  apply unique_list_vector in H1.
+  simpl in *.
+  exact H1.
+Qed.
+
+Theorem cast_o_cvir_unique :
+  forall ni no no' (ir : cvir ni no) (H : no = no'),
+  unique_bid ir -> unique_bid (cast_o_cvir ir H).
+Proof.
+  unfold unique_bid. intros.
+  simpl in *.
+  eapply H0 ; try eassumption.
+Qed.
+
+Theorem focus_input_cvir_id_WF :
+  forall ni no (ir : cvir ni no) (i : fin ni),
+  cvir_ids_WF ir -> cvir_ids_WF (focus_input_cvir ir i).
+Proof.
+  unfold focus_input_cvir.
+  intros.
+  apply cast_i_cvir_id_WF.
+  apply sym_i_cvir_id_WF.
+  apply cast_i_cvir_id_WF.
+  apply sym_i_cvir_id_WF.
+  apply cast_i_cvir_id_WF.
+  exact H.
+Qed.
+
+Theorem focus_input_cvir_unique :
+  forall ni no (ir : cvir ni no) (i : fin ni),
+  unique_bid ir -> unique_bid (focus_input_cvir ir i).
+Proof.
+  unfold focus_input_cvir.
+  intros.
+  apply cast_i_cvir_unique.
+  apply sym_i_cvir_unique.
+  apply cast_i_cvir_unique.
+  apply sym_i_cvir_unique.
+  apply cast_i_cvir_unique.
+  exact H.
+Qed.
+
+Theorem loop_cvir_open_id_WF :
+  forall (ni no : nat) (ir : cvir (S ni) (S no)),
+  cvir_ids_WF ir -> cvir_ids_WF (loop_cvir_open ir).
+Proof.
+  unfold loop_cvir_open.
+  unfold cvir_ids_WF.
+  intros.
+  simpl in *.
+  specialize (H vi (hd vi :: vo) vt b).
+  intuition.
+  specialize (H2 _ H1).
+  apply in_app_iff in H2. simpl in H2. apply in_app_iff.
+  intuition.
+  subst.
+Admitted.
+
+Theorem loop_cvir_id_WF :
+  forall (ni no : nat) (ir : cvir (S ni) (S no)),
+  cvir_ids_WF ir -> cvir_ids_WF (loop_cvir ir).
+Proof.
+  unfold loop_cvir.
+  unfold cvir_ids_WF.
+  intros.
+  simpl in *.
+  destruct (uncons vt) eqn:? in H0.
+  apply cons_uncons in Heqp. subst vt.
+  specialize (H (r::vi) (r::vo) t b).
+  apply H in H0.
+  split.
+  - destruct H0 as [H0 _].
+    apply in_app_iff.
+    apply in_app_iff in H0.
+    simpl in *.
+    tauto.
+  - destruct H0 as [_ H0].
+    intros. specialize (H0 bid H1).
+    apply in_app_iff.
+    apply in_app_iff in H0.
+    simpl in *.
+    tauto.
+Qed.
+
+Theorem loop_cvir_unique :
+  forall (ni no : nat) (ir : cvir (S ni) (S no)),
+  unique_bid ir -> unique_bid (loop_cvir ir).
+Proof.
+  unfold loop_cvir, unique_bid.
+  intros.
+  simpl in *.
+  destruct (uncons vt) eqn:? in H1, H2.
+  apply cons_uncons in Heqp. subst vt.
+  eapply H ; try eassumption.
+  apply unique_list_vector. apply unique_list_vector in H0. simpl in *.
+  replace (r :: proj1_sig t)%list with ((r :: nil) ++ proj1_sig t)%list in H0 by reflexivity.
+  apply unique_list_sym in H0.
+  rewrite <- app_assoc in H0.
+  apply unique_list_sym2 in H0.
+  apply H0.
+Qed.
+
 Theorem seq_cvir_id_WF :
   forall ni1 no1 ni2 no2 (ir1 : cvir ni1 (S no1)) (ir2 : cvir (S ni2) no2),
   cvir_ids_WF ir1 -> cvir_ids_WF ir2 ->
   cvir_ids_WF (seq_cvir ir1 ir2).
 Proof.
-  unfold cvir_ids_WF.
+  unfold seq_cvir.
   intros.
-  split_vec vi ni1.
-  split_vec vo no1.
-  simpl in *.
-  destruct (Vec.uncons vt) as [it vt'] eqn:?.
-  apply cons_uncons in Heqp. subst.
-  split_vec vt' (n_int ir1).
-  rewrite 2 splitat_append.
-  edestruct H, H0.
-  split.
-  - intro.
-    apply in_app_iff in H5.
-    rewrite 2 vector_in_app_iff.
-    unfold In. simpl.
-    destruct H5 ; apply H1 in H5 + apply H3 in H5 ; apply in_app_iff in H5 ; simpl in * ; intuition.
-  - intros.
-    rewrite 2 vector_in_app_iff.
-    unfold In. simpl.
-    apply in_app_iff in H5.
-    destruct H5 ; eapply H2 in H5 + eapply H4 in H5; try eassumption ;
-    apply vector_in_app_iff in H5 ; unfold In in H5 ; simpl in H5 ; intuition.
+  apply loop_cvir_id_WF.
+  apply cast_o_cvir_id_WF.
+  apply cast_i_cvir_id_WF.
+  apply focus_input_cvir_id_WF.
+  apply merge_cvir_id_WF ; assumption.
 Qed.
-
-  (*intros.
-  unfold cvir_ids_WF.
-  intros.
-  Opaque merge_cvir.
-  simpl.
-  split.
-  - assert (H1 := merge_cvir_id_WF _ _ _ _ ir1 ir2 H H0).
-    unfold cvir_ids_WF in H1.
-    destruct (Vec.uncons vt) as [it vt'] eqn:?.
-    apply cons_uncons in Heqp. subst.
-    assert (List.In b
-  (blocks
-     (merge_cvir
-        (mk_cvir
-           (fun (vi0 : Vec.t raw_id ni1) (vo0 : Vec.t raw_id no1) (vt0 : Vec.t raw_id (n_int ir1)) =>
-            blocks ir1 vi0 (it :: vo0) vt0))
-        (mk_cvir
-           (fun (vi0 : Vec.t raw_id ni2) (vo0 : Vec.t raw_id no2) (vt0 : Vec.t raw_id (n_int ir2)) =>
-            blocks ir2 (it :: vi0) vo0 vt0))) vi vo vt') -> In (blk_id b) (vi ++ vt')).
-    apply merge_cvir_id_WF.
-    admit. admit.
-    intro.
-    apply Coqlib.list_in_insert.
-    specialize (H2 H3).
-    assumption.*)
 
 Theorem seq_cvir_unique :
   forall ni1 no1 ni2 no2 (ir1 : cvir ni1 (S no1)) (ir2 : cvir (S ni2) no2),
-  cvir_ids_WF ir1 ->
-  cvir_ids_WF ir2 ->
-  unique_bid ir1 ->
-  unique_bid ir2 ->
+  cvir_ids_WF ir1 -> cvir_ids_WF ir2 ->
+  unique_bid ir1 -> unique_bid ir2 ->
   unique_bid (seq_cvir ir1 ir2).
 Proof.
-  intros.
   unfold seq_cvir.
-  Opaque merge_cvir.
-  simpl.
-  unfold unique_bid in *.
   intros.
-  split_vec vi ni1.
-  split_vec vo no1.
-  simpl in *.
-  destruct (Vec.uncons vt) as [it vt'] eqn:?.
-  apply cons_uncons in Heqp. subst.
-  split_vec vt' (n_int ir1).
-  eapply merge_cvir_unique. 6: eassumption. 6: eassumption. all: eauto.
-Admitted.
+  apply loop_cvir_unique.
+  apply cast_o_cvir_unique.
+  apply cast_i_cvir_unique.
+  apply focus_input_cvir_unique.
+  apply merge_cvir_unique ; assumption.
+Qed.
