examples/Imp2Vir/Unique.v
@@ -84,6 +84,18 @@ Proof.
     reflexivity.
 Qed.
 
+Theorem unique_vector_assoc :
+  forall A n1 n2 n3 (v1 : Vec.t A n1) (v2 : Vec.t A n2) (v3 : Vec.t A n3),
+  unique_vector (v1 ++ v2 ++ v3)%vec -> unique_vector ((v1 ++ v2) ++ v3)%vec.
+Proof.
+  intros.
+  apply unique_list_vector.
+  apply unique_list_vector in H.
+  simpl in *.
+  rewrite <- app_assoc.
+  exact H.
+Qed.
+
 Theorem unique_vector_sym : forall A n1 n2 (v1 : Vec.t A n1) (v2 : Vec.t A n2),
   unique_vector (v1 ++ v2)%vec -> unique_vector (v2 ++ v1)%vec.
 Proof.
